Sync

coq/theories/imp2asm/ImpToASMCodegen.v
@@ -110,20 +110,27 @@ Function index_of_opt (n : name) (k : nat) (vs : v_stack) : option nat :=
 
 (* lookup variable with name `n`, based on stack `vs` *)
 Definition c_var (n : name) (l : nat) (vs : v_stack) : asm_appl * nat :=
-  letd k := (index_of n 0 vs) in
+  let/d k := (index_of n 0 vs) in
   if k =? 0 then (List [ASMSyntax.Push RAX], l+1)
   else (List [ASMSyntax.Push RAX; ASMSyntax.Load_RSP RAX k], l+2).
 
+Fixpoint c_declare_binders_rec (binders: list name) (l: nat) (vs: v_stack) (acc_asm: asm_appl): (asm_appl * nat * v_stack) :=
+  match binders with
+  | nil => (acc_asm, l, vs)
+  | binder_name :: binders =>
+    c_declare_binders_rec binders (l + 1) ((Some binder_name) :: vs) (acc_asm +++ List [ASMSyntax.Push RDI])
+  end.
+
+Definition c_declare_binders (binders: list name) (l: nat) (vs: v_stack): (asm_appl * nat * v_stack) :=
+  let/d '(asm1, l1, vs1) := c_declare_binders_rec binders (l + 1) vs (List []) in
+  (asm1 +++ List [ASMSyntax.Const RDI (word.of_Z 0)], l1, vs1).
+
 (* assign variable with name `n`, based on stack *)
-Definition c_assign (n : name) (l : nat) (vs : v_stack) : (asm_appl * nat * v_stack) :=
-  letd k := (index_of_opt n 0 vs) in
-  match k return (asm_appl * nat * v_stack) with
-  | None => (List [], l, (Some n) :: vs)
-  | Some kv =>
-    match kv with
-    | 0 => (List [ASMSyntax.Pop RDI], l+1, vs)
-    | S _ => (List [ASMSyntax.Store_RSP RAX kv; ASMSyntax.Pop RAX], l+2, vs)
-    end
+Definition c_assign (n : name) (l : nat) (vs : v_stack) : (asm_appl * nat) :=
+  let/d k := index_of n 0 vs in
+  match k return (asm_appl * nat) with
+  | 0 => (List [ASMSyntax.Pop RDI], l+1)
+  | S _ => (List [ASMSyntax.Store_RSP RAX k; ASMSyntax.Pop RAX], l+2)
   end.
 
 (*
@@ -165,11 +172,11 @@ Definition align (needs_alignment : bool) (asm1 : asm_appl) : asm_appl :=
   if needs_alignment then (List [Push RAX]) +++ asm1 +++ (List [Pop RDI]) else asm1.
 
 Definition c_read (vs : v_stack) (l : nat) : (asm_appl * nat) :=
-  letd asm1 := align (even_len vs) (List [ASMSyntax.Push RAX; ASMSyntax.GetChar]) in
+  let/d asm1 := align (even_len vs) (List [ASMSyntax.Push RAX; ASMSyntax.GetChar]) in
   (asm1, l + app_list_length asm1).
 
 Definition c_write (vs : v_stack) (l : nat) : (asm_appl * nat) :=
-  letd asm1 := align (even_len vs) (List [Mov RDI RAX; ASMSyntax.PutChar; ASMSyntax.Const RAX (word.of_Z 0)]) in
+  let/d asm1 := align (even_len vs) (List [Mov RDI RAX; ASMSyntax.PutChar; ASMSyntax.Const RAX (word.of_Z 0)]) in
   (asm1, l + app_list_length asm1).
 
 (*
@@ -202,22 +209,22 @@ Function c_exp (e : exp) (l : nat) (vs : v_stack) : asm_appl * nat :=
   | Var n => c_var n l vs
   | Const n => c_const n l vs
   | Add e1 e2 =>
-      letd '(asm1, l1) := c_exp e1 l vs in
-      letd '(asm2, l2) := c_exp e2 l1 (None :: vs) in
-      letd c_add_asm := c_add (None :: None :: vs) in
+      let/d '(asm1, l1) := c_exp e1 l vs in
+      let/d '(asm2, l2) := c_exp e2 l1 (None :: vs) in
+      let/d c_add_asm := c_add (None :: None :: vs) in
       (asm1 +++ asm2 +++ c_add_asm, l2 + app_list_length c_add_asm)
   | Sub e1 e2 =>
-      letd '(asm1, l1) := c_exp e1 l vs in
-      letd '(asm2, l2) := c_exp e2 l1 (None :: vs) in
-      letd c_sub_asm := c_sub l2 in
+      let/d '(asm1, l1) := c_exp e1 l vs in
+      let/d '(asm2, l2) := c_exp e2 l1 (None :: vs) in
+      let/d c_sub_asm := c_sub l2 in
       (asm1 +++ asm2 +++ c_sub_asm, l2 + app_list_length c_sub_asm)
   | Div e1 e2 =>
-      letd '(asm1, l1) := c_exp e1 l vs in
-      letd '(asm2, l2) := c_exp e2 l1 (None :: vs) in
+      let/d '(asm1, l1) := c_exp e1 l vs in
+      let/d '(asm2, l2) := c_exp e2 l1 (None :: vs) in
       (asm1 +++ asm2 +++ c_div, l2 + app_list_length c_div)
   | Read e1 e2 =>
-      letd '(asm1, l1) := c_exp e1 l vs in
-      letd '(asm2, l2) := c_exp e2 l1 (None :: vs) in
+      let/d '(asm1, l1) := c_exp e1 l vs in
+      let/d '(asm2, l2) := c_exp e2 l1 (None :: vs) in
       (asm1 +++ asm2 +++ c_load, l2 + app_list_length c_load)
   end.
 
@@ -225,8 +232,8 @@ Function c_exps (es: list exp) (l : nat) (vs : v_stack) : asm_appl * nat :=
   match es with
   | [] => (List [], l)
   | e :: es' =>
-    letd '(asm1, l1) := c_exp e l vs in
-    letd '(asm2, l2) := c_exps es' l1 vs in
+    let/d '(asm1, l1) := c_exp e l vs in
+    let/d '(asm2, l2) := c_exps es' l1 vs in
     (asm1 +++ asm2, l2)
   end.
 
@@ -243,23 +250,23 @@ Function c_test_jump (t : test) (pos_label : nat) (neg_label : nat)
   (l : nat) (vs : v_stack) : asm_appl * nat :=
   match t with
   | Test c e1 e2 =>
-    letd '(asm1, l1) := c_exp e1 l vs in
-    letd '(asm2, l2) := c_exp e2 l1 (None :: vs) in
-    letd c_cmp_asm := List [Mov RBX RAX; Pop RDI; Pop RAX;
+    let/d '(asm1, l1) := c_exp e1 l vs in
+    let/d '(asm2, l2) := c_exp e2 l1 (None :: vs) in
+    let/d c_cmp_asm := List [Mov RBX RAX; Pop RDI; Pop RAX;
       ASMSyntax.Jump (c_cmp c) pos_label;
       ASMSyntax.Jump Always neg_label] in
     (asm1 +++ asm2 +++ c_cmp_asm, l2 + app_list_length c_cmp_asm)
   | And t1 t2 =>
-    letd '(asm1, l1) := c_test_jump t1 (l + 1) neg_label (l + 2) vs in
-    letd '(asm2, l2) := c_test_jump t2 pos_label neg_label l1 vs in
-    letd jump_to_start := List [ASMSyntax.Jump Always (l + 2)] in
-    letd jump_to_t2 := List [ASMSyntax.Jump Always l1] in (* l1 is the start of t2*)
+    let/d '(asm1, l1) := c_test_jump t1 (l + 1) neg_label (l + 2) vs in
+    let/d '(asm2, l2) := c_test_jump t2 pos_label neg_label l1 vs in
+    let/d jump_to_start := List [ASMSyntax.Jump Always (l + 2)] in
+    let/d jump_to_t2 := List [ASMSyntax.Jump Always l1] in (* l1 is the start of t2*)
     (jump_to_start +++ jump_to_t2 +++ asm1 +++ asm2, l2)
   | Or t1 t2 =>
-    letd '(asm1, l1) := c_test_jump t1 pos_label (l + 1) (l + 2) vs in
-    letd '(asm2, l2) := c_test_jump t2 pos_label neg_label l1 vs in
-    letd jump_to_start := List [ASMSyntax.Jump Always (l + 2)] in
-    letd jump_to_t2 := List [ASMSyntax.Jump Always l1] in (* l1 is the start of t2*)
+    let/d '(asm1, l1) := c_test_jump t1 pos_label (l + 1) (l + 2) vs in
+    let/d '(asm2, l2) := c_test_jump t2 pos_label neg_label l1 vs in
+    let/d jump_to_start := List [ASMSyntax.Jump Always (l + 2)] in
+    let/d jump_to_t2 := List [ASMSyntax.Jump Always l1] in (* l1 is the start of t2*)
     (jump_to_start +++ jump_to_t2 +++ asm1 +++ asm2, l2)
   | Not t' =>
     c_test_jump t' neg_label pos_label l vs
@@ -280,7 +287,7 @@ Definition make_ret (vs : v_stack) (l : nat) : asm_appl * nat :=
 (* Store the variables from the stack in the registers, so that they can be
 passed to the function call *)
 Definition c_pops (xs : list exp) (vs : v_stack) : asm_appl :=
-  letd k := List.length xs in
+  let/d k := List.length xs in
   if k =? 0 then List [Push RAX] else
   if k =? 1 then List [] else
   if k =? 2 then List [Pop RDI] else
@@ -298,8 +305,8 @@ Function call_v_stack (xs: list name) (acc: v_stack): v_stack :=
 
 (** Push a list of variables onto the stack *)
 Definition c_pushes (v_names: list name) (l : nat): (asm_appl * v_stack * nat) :=
-  letd k := List.length v_names in
-  letd e := call_v_stack v_names [] in
+  let/d k := List.length v_names in
+  let/d e := call_v_stack v_names [] in
   if k =? 0 then (List [], [None], l) else
   if k =? 1 then (List [], e, l) else
   if k =? 2 then (List [Push RDI], e, l + 1) else
@@ -310,83 +317,115 @@ Definition c_pushes (v_names: list name) (l : nat): (asm_appl * v_stack * nat) :
 (* Call the given function, passing the arguments in registers*)
 Definition c_call (vs : v_stack) (target : nat)
   (xs : list exp) (l : nat) : asm_appl * nat :=
-  letd asm_pops := c_pops xs vs in
-  letd asm1 := align (even_len vs) (List [ASMSyntax.Call target]) in
+  let/d asm_pops := c_pops xs vs in
+  let/d asm1 := align (even_len vs) (List [ASMSyntax.Call target]) in
   (asm_pops +++ asm1, l + app_list_length asm_pops + app_list_length asm1).
 
-Function c_cmd (c : cmd) (l : nat) (fs : f_lookup)
-  (vs : v_stack) : (asm_appl * nat * v_stack) :=
+Function c_cmd (c : cmd) (l : nat) (fs : f_lookup) (vs : v_stack) : (asm_appl * nat) :=
   match c with
   | Seq c1 c2 =>
-    letd '(asm1, l1, vs1) := c_cmd c1 l fs vs in
-    letd '(asm2, l2, vs2) := c_cmd c2 l1 fs vs1 in
-    (asm1 +++ asm2, l2, vs2)
+    let/d '(asm1, l1) := c_cmd c1 l fs vs in
+    let/d '(asm2, l2) := c_cmd c2 l1 fs vs in
+    (asm1 +++ asm2, l2)
   | Assign n e =>
-    letd '(asm1, l1) := c_exp e l vs in
-    letd '(asm2, l2, vs2) := c_assign n l1 vs in
-    (asm1 +++ asm2, l2, vs2)
+    let/d '(asm1, l1) := c_exp e l vs in
+    let/d '(asm2, l2) := c_assign n l1 vs in
+    (asm1 +++ asm2, l2)
   | Update a e e' =>
-    letd '(asm1, l1) := c_exp a l vs in
-    letd '(asm2, l2) := c_exp e l1 vs in
-    letd '(asm3, l3) := c_exp e' l2 (None :: vs) in
-    letd asm4 := c_store in
-    (asm1 +++ asm2 +++ asm3 +++ asm4, l3 + app_list_length asm4, vs)
+    let/d '(asm1, l1) := c_exp a l vs in
+    let/d '(asm2, l2) := c_exp e l1 vs in
+    let/d '(asm3, l3) := c_exp e' l2 (None :: vs) in
+    let/d asm4 := c_store in
+    (asm1 +++ asm2 +++ asm3 +++ asm4, l3 + app_list_length asm4)
   | If t c1 c2 =>
-    letd '(asm1, l1) := c_test_jump t (l + 1) (l + 2) (l + 3) vs in
-    letd '(asm2, l2, vs2) := c_cmd c1 l1 fs vs in
-    letd '(asm3, l3, vs3) := c_cmd c2 (l2 + 1) fs vs in
-    letd jump_to_start := List[ASMSyntax.Jump Always (l + 3)] in
-    letd jump_to_c1 := List [ASMSyntax.Jump Always l1] in
-    letd jump_to_c2 := List [ASMSyntax.Jump Always l2] in
-    letd jump_to_end := List [ASMSyntax.Jump Always l3] in
-    letd asmres := jump_to_start +++ jump_to_c1 +++ jump_to_c2 +++ asm1 +++ asm2 +++ jump_to_end +++ asm3 in
+    let/d '(asm1, l1) := c_test_jump t (l + 1) (l + 2) (l + 3) vs in
+    let/d '(asm2, l2) := c_cmd c1 l1 fs vs in
+    let/d '(asm3, l3) := c_cmd c2 (l2 + 1) fs vs in
+    let/d jump_to_start := List[ASMSyntax.Jump Always (l + 3)] in
+    let/d jump_to_c1 := List [ASMSyntax.Jump Always l1] in
+    let/d jump_to_c2 := List [ASMSyntax.Jump Always l2] in
+    let/d jump_to_end := List [ASMSyntax.Jump Always l3] in
+    let/d asmres := jump_to_start +++ jump_to_c1 +++ jump_to_c2 +++ asm1 +++ asm2 +++ jump_to_end +++ asm3 in
     (* TODO(kπ): Cannot know the result `vs` statically. Is there a better way to compile `if`s? *)
     (*           Should we manually drop the additional stuff from the stack *)
-    (asmres, l3, vs)
+    (asmres, l3)
   | While tst body =>
-    letd '(asm1, l1) := c_test_jump tst (l + 1) (l + 2) (l + 3) vs in
-    letd '(asm2, l2, vs2) := c_cmd body l1 fs vs in
-    letd jump_to_tst := List [ASMSyntax.Jump Always (l + 3)] in
-    letd jump_to_beginning := List [ASMSyntax.Jump Always l] in
-    letd jump_to_body := List [ASMSyntax.Jump Always l1] in
-    letd jump_to_end := List [ASMSyntax.Jump Always (l2 + 1)] in
-    letd asmres := jump_to_tst +++ jump_to_body +++ jump_to_end +++ asm1 +++ asm2 +++ jump_to_beginning in
+    let/d '(asm1, l1) := c_test_jump tst (l + 1) (l + 2) (l + 3) vs in
+    let/d '(asm2, l2) := c_cmd body l1 fs vs in
+    let/d jump_to_tst := List [ASMSyntax.Jump Always (l + 3)] in
+    let/d jump_to_beginning := List [ASMSyntax.Jump Always l] in
+    let/d jump_to_body := List [ASMSyntax.Jump Always l1] in
+    let/d jump_to_end := List [ASMSyntax.Jump Always (l2 + 1)] in
+    let/d asmres := jump_to_tst +++ jump_to_body +++ jump_to_end +++ asm1 +++ asm2 +++ jump_to_beginning in
     (* TODO(kπ): Same as with if: what's the correct result `vs` here? *)
-    (asmres, l2+1, vs)
+    (asmres, l2+1)
   | Call n f es =>
-    letd target := lookup f fs in
-    letd '(asms, l1) := c_exps es l vs in
-    letd '(asm1, l2) := c_call vs target es l1 in
-    letd '(asm2, l3) := c_var n l2 vs in
-    (asms +++ asm1 +++ asm2, l3, vs)
+    let/d target := lookup f fs in
+    let/d '(asms, l1) := c_exps es l vs in
+    let/d '(asm1, l2) := c_call vs target es l1 in
+    let/d '(asm2, l3) := c_var n l2 vs in
+    (asms +++ asm1 +++ asm2, l3)
   | Return e =>
-    letd '(asm1, l1) := c_exp e l vs in
-    letd '(asm2, l2) := make_ret vs l1 in
-    (asm1 +++ asm2, l2, vs)
+    let/d '(asm1, l1) := c_exp e l vs in
+    let/d '(asm2, l2) := make_ret vs l1 in
+    (asm1 +++ asm2, l2)
   | Alloc n e =>
-    letd '(asm1, l1) := c_exp e l vs in
-    letd asm2 := c_alloc vs in
-    letd '(asm3, l3, vs3) := c_assign n (l1 + app_list_length asm2) vs in
-    (asm1 +++ asm2 +++ asm3, l3, vs3)
+    let/d '(asm1, l1) := c_exp e l vs in
+    let/d asm2 := c_alloc vs in
+    let/d '(asm3, l3) := c_assign n (l1 + app_list_length asm2) vs in
+    (asm1 +++ asm2 +++ asm3, l3)
   | GetChar n =>
-    letd '(asm1, l1) := c_read vs l in
-    letd '(asm2, l2, vs2) := c_assign n l1 vs in
-    (asm1 +++ asm2, l2, vs2)
+    let/d '(asm1, l1) := c_read vs l in
+    let/d '(asm2, l2) := c_assign n l1 vs in
+    (asm1 +++ asm2, l2)
   | PutChar e =>
-    letd '(asm1, l1) := c_exp e l vs in
-    letd '(asm2, l2) := c_write vs l1 in
-    (asm1 +++ asm2, l2, vs)
+    let/d '(asm1, l1) := c_exp e l vs in
+    let/d '(asm2, l2) := c_write vs l1 in
+    (asm1 +++ asm2, l2)
   | Abort =>
-    (List [Jump Always (abort (odd_len vs))], l+1, vs)
+    (List [Jump Always (abort (odd_len vs))], l+1)
   end.
+
+Fixpoint all_binders (body: cmd): list name :=
+  match body with
+  | Seq c1 c2 => all_binders c1 ++ all_binders c2
+  | Assign n e => [n]
+  | Update a e e' => []
+  | If t c1 c2 => all_binders c1 ++ all_binders c2
+  | While tst body => all_binders body
+  | Call n f es => [n]
+  | Return e => []
+  | Alloc n e => [n]
+  | GetChar n => [n]
+  | PutChar e => []
+  | Abort => []
+  end.
+
+Fixpoint names_contain (l: list name) (a: name): bool :=
+  match l with
+  | nil => false
+  | x :: l => (x =? a) || names_contain l a
+  end.
+
+Fixpoint names_unique (l: list name) (acc: list name): list name :=
+  match l with
+  | nil => acc
+  | x :: l => names_unique l (if names_contain acc x then acc else (x :: acc))
+  end.
+
+Definition unique_binders (body: cmd): list name :=
+  let/d binds := all_binders body in
+  names_unique binds [].
 
 (** Compiles a single function definition into assembly code. *)
 Definition c_fundef (fundef : func) (l: nat) (fs: f_lookup): (asm_appl * nat) :=
   match fundef with
   | Func n v_names body =>
-    letd '(asm0, vs0, l0) := c_pushes v_names l in
-    letd '(asm1, l1, vs1) := c_cmd body l0 fs vs0 in
-    (asm0 +++ asm1, l1)
+    let/d '(asm0, vs0, l0) := c_pushes v_names l in
+    let/d binders := unique_binders body in
+    let/d '(asm1, l1, vs1) := c_declare_binders binders l0 vs0 in
+    let/d '(asm2, l2) := c_cmd body l0 fs vs1 in
+    (asm0 +++ asm1 +++ asm2, l2)
   end.
 
 (* TODO(kπ) termination is unobvious to Coq, super unimportant function, hacked for now *)
@@ -405,10 +444,10 @@ Function c_fundefs (ds : list func) (l : nat) (fs : f_lookup) : (asm_appl * list
   match ds with
   | [] => (List [], fs, l)
   | d :: ds' =>
-    letd fname := name_of_func d in
-    letd comment := List [Comment (name2str fname "")] in
-    letd '(c1, l1) := c_fundef d (l + 1) fs in
-    letd '(c2, fs', l2) := c_fundefs ds' l1 fs in
+    let/d fname := name_of_func d in
+    let/d comment := List [Comment (name2str fname "")] in
+    let/d '(c1, l1) := c_fundef d (l + 1) fs in
+    let/d '(c2, fs', l2) := c_fundefs ds' l1 fs in
     (comment +++ c1 +++ c2, (fname, l + 1) :: fs', l2)
   end.
 
@@ -417,9 +456,9 @@ Definition lookup_main (fs : f_lookup) : nat :=
 
 (* Generates the complete assembly code for a given program *)
 Definition codegen (prog : prog) : asm :=
-  letd funs := get_funcs prog in
-  letd init_l := app_list_length (List (init 0)) in
-  letd '(_, fs, _) := c_fundefs funs init_l [] in
-  letd '(asm1, _, _) := c_fundefs funs init_l fs in
-  letd main_l := lookup_main fs in
+  let/d funs := get_funcs prog in
+  let/d init_l := app_list_length (List (init 0)) in
+  let/d '(_, fs, _) := c_fundefs funs init_l [] in
+  let/d '(asm1, _, _) := c_fundefs funs init_l fs in
+  let/d main_l := lookup_main fs in
   flatten ((List (init main_l)) +++ asm1).
